Bitcoin/Zord.v
@@ -1,0 +1,71 @@
+From mathcomp.ssreflect
+Require Import ssreflect ssrbool ssrnat eqtype ssrfun seq fintype path.
+Require Import Eqdep.
+From HTT
+Require Import pred prelude idynamic ordtype pcm finmap unionmap heap.
+Require Import ZArith.
+Set Implicit Arguments.
+Unset Strict Implicit.
+Unset Printing Implicit Defensive.
+
+Section ZOrd.
+
+Open Scope Z_scope.
+
+Lemma eqZP : Equality.axiom Z_eq_dec.
+Proof.
+move => x y.
+by apply: (iffP idP); case Z_eq_dec.
+Qed.
+
+Canonical Z_eqMixin := EqMixin eqZP.
+Canonical Z_eqType := Eval hnf in EqType Z Z_eqMixin.
+
+Lemma ZltP :
+  forall x y, reflect (x < y) (Z_lt_dec x y).
+Proof.
+by move => x y; apply: (iffP idP); case Z_lt_dec.
+Qed.
+
+Lemma irr_Z_lt_dec : irreflexive Z_lt_dec.
+Proof.
+move => x.
+apply/ZltP.
+exact: Z.lt_irrefl.
+Qed.
+
+Lemma trans_Z_lt_dec : transitive Z_lt_dec.
+Proof.
+move => x y z.
+move/ZltP => H_lt1.
+move/ZltP => H_lt2.
+apply/ZltP.
+move: H_lt1 H_lt2.
+exact: Z.lt_trans.
+Qed.
+
+Lemma total_Z_lt_dec : forall x y, [|| Z_lt_dec x y, x == y | Z_lt_dec y x].
+Proof.
+move => x y.
+case (Z_dec x y) => H_dec.
+- case: H_dec => H_dec.
+  * apply/orP.
+    left.
+    by apply/ZltP.
+  * apply/orP.
+    right.
+    apply/orP.
+    right.
+    apply/ZltP.
+    by auto with zarith.
+- apply/orP.
+  right.
+  apply/orP.
+  left.
+  by apply/eqZP.
+Qed.
+
+Definition Z_ordMixin := OrdMixin irr_Z_lt_dec trans_Z_lt_dec total_Z_lt_dec.
+Canonical Structure Z_ordType := OrdType Z Z_ordMixin.
+
+End ZOrd.
